# baseURI: http://linked.data.gov.au/def/geox
# imports: http://linked.data.gov.au/def/datatype
# imports: http://www.opengis.net/ont/geosparql
# prefix: geox

@prefix data: <http://linked.data.gov.au/def/datatype/> .
@prefix dcterms: <http://purl.org/dc/terms/> .
@prefix geo: <http://www.opengis.net/ont/geosparql#> .
@prefix geox: <http://linked.data.gov.au/def/geox#> .
@prefix owl: <http://www.w3.org/2002/07/owl#> .
@prefix rdf: <http://www.w3.org/1999/02/22-rdf-syntax-ns#> .
@prefix rdfs: <http://www.w3.org/2000/01/rdf-schema#> .
@prefix sdo: <https://schema.org/> .
@prefix skos: <http://www.w3.org/2004/02/skos/core#> .
@prefix xsd: <http://www.w3.org/2001/XMLSchema#> .

<http://linked.data.gov.au/def/geox>
  a owl:Ontology ;
  dcterms:created "2019-01-08"^^xsd:date ;
  dcterms:creator <https://orcid.org/0000-0002-3884-3420> ;
  dcterms:creator <https://orcid.org/0000-0002-8742-7730> ;
  dcterms:modified "2020-06-24"^^xsd:date ;
  dcterms:publisher <https://ror.org/03qn8fb07> ;
  dcterms:requires <http://linked.data.gov.au/def/datatype> ;
  dcterms:requires <http://qudt.org/2.1/vocab/unit> ;
  dcterms:requires <http://www.opengis.net/ont/geosparql> ;
  rdfs:comment "An extension to [GeoSPARQL](http://www.opengeospatial.org/standards/geosparql) with new features for the representation of additional elements of feature geometry, such as spatial-resolution, length, area and volume. " ;
  rdfs:label "GeoSPARQL Extensions Ontology"@en ;
  rdfs:seeAlso <https://github.com/CSIRO-enviro-informatics/geosparql-ext-ont> ;
  owl:imports <http://linked.data.gov.au/def/datatype> ;
  owl:imports <http://www.opengis.net/ont/geosparql> ;
  owl:versionIRI <http://linked.data.gov.au/def/geox/1.1> ;
  skos:changeNote "Added BBox" ;
  skos:changeNote "This iteration uses the AGLDWG data-types vocabulary for quantities. " ;
  skos:editorialNote "The specific elements of this ontology have been created to facilitate use cases generated by the [LocI project](http://loci.cat).These elements will be submitted for consideration for future editions of the GeoSPARQL ontology." ;
  sdo:codeRepository <https://github.com/CSIRO-enviro-informatics/geosparql-ext-ont> ;
.
geox:BBox
  a owl:Class ;
  rdfs:comment """The two corners shodul be specified using the same CRS. 

The edges/faces of the box align with the axes of the CRS used for the corners.""" ;
  rdfs:label "Bounding box" ;
  rdfs:subClassOf geo:Geometry ;
  rdfs:subClassOf [
      a owl:Restriction ;
      owl:cardinality "1"^^xsd:nonNegativeInteger ;
      owl:onProperty geox:lowerLeft ;
    ] ;
  rdfs:subClassOf [
      a owl:Restriction ;
      owl:cardinality "1"^^xsd:nonNegativeInteger ;
      owl:onProperty geox:upperRight ;
    ] ;
  skos:example """
ex:BB99
      rdf:type geox:BBox ;
      geox:lowerLeft \"<http://www.opengis.net/def/crs/OGC/1.3/CRS84> POINT(138 -29.5)\"^^geo:wktLiteral ;
      geox:upperRight \"<http://www.opengis.net/def/crs/OGC/1.3/CRS84> POINT(155 -9)\"^^geo:wktLiteral ;
.

ex:BB88
      rdf:type geox:BBox ;
      geox:lowerLeft \"{\\\"type\\\":\\\"Point\\\",\\\"coordinates\\\":[138, -29.179266]}\"^^rdf:JSON ;
      geox:upperRight \"{\\\"type\\\":\\\"Point\\\",\\\"coordinates\\\":[153.577908, -8.998516]}\"^^rdf:JSON ;
.""" ;
.
geox:SpatialMeasure
  a owl:Class ;
  rdfs:label "Spatial measure" ;
  rdfs:subClassOf data:QuantitativeMeasure ;
  rdfs:subClassOf [
      a owl:Restriction ;
      owl:cardinality "1"^^xsd:nonNegativeInteger ;
      owl:onProperty geox:inCRS ;
    ] ;
  skos:definition "Scalar quantity computed or defined within a specified coordinate reference system" ;
  skos:example """
ex:Area20858M2 
      rdf:type geox:SpatialMeasure ;
      data:value 4185791.9328826475 ;
      geox:inCRS <http://www.opengis.net/def/crs/EPSG/0/3857> ;
.
""" ;
.
geox:hasArea
  a owl:ObjectProperty ;
  rdfs:domain geo:SpatialObject ;
  rdfs:label "has area" ;
  rdfs:range geox:SpatialMeasure ;
  skos:definition "The area of a spatial object, expressed as a scaled number" ;
  skos:example """
auspix:R7430551
  rdf:type geo:Feature ;
  geox:hasArea [
      data:uncertainty 1.5 ;
      data:unit <http://qudt.org/vocab/unit/M2> ;
      data:value 17793623.0 ;
    ] ;
  geo:hasGeometry [
    rdf:type sf:Polygon ;
    geo:asWKT \"POLYGON((131.02880658436214 -25.331112553792963 , 131.06995884773661 -25.331112553792963  , 131.06995884773661 -25.36980468021464 , 131.02880658436214 -25.36980468021464 , 131.02880658436214 -25.331112553792963))\"^^geo:wktLiteral ;
    ] ;
  rdfs:seeAlso <http://ec2-52-63-73-113.ap-southeast-2.compute.amazonaws.com/AusPIX-DGGS-dataset/ausPIX/R7430551> ;
.""" ;
.
geox:hasAreaM2
  a owl:ObjectProperty ;
  rdfs:label "has area in m2" ;
  rdfs:range [
      a owl:Class ;
      rdfs:subClassOf geox:SpatialMeasure ;
      rdfs:subClassOf [
          a owl:Restriction ;
          owl:hasValue <http://qudt.org/vocab/unit/M2> ;
          owl:onProperty data:unit ;
        ] ;
    ] ;
  rdfs:subPropertyOf geox:hasArea ;
  skos:definition "The area of the spatial object in m^2" ;
  skos:example """
auspix:R7430551
  rdf:type geo:Feature ;
  geox:hasAreaM2 [
      data:value 17793623.0 ;
    ] ;
  geo:hasGeometry [
    rdf:type sf:Polygon ;
    geo:asWKT \"POLYGON((131.02880658436214 -25.331112553792963 , 131.06995884773661 -25.331112553792963  , 131.06995884773661 -25.36980468021464 , 131.02880658436214 -25.36980468021464 , 131.02880658436214 -25.331112553792963))\"^^geo:wktLiteral ;
  ] ;
  rdfs:seeAlso <http://ec2-52-63-73-113.ap-southeast-2.compute.amazonaws.com/AusPIX-DGGS-dataset/ausPIX/R7430551> ;
.""" ;
.
geox:hasBBox
  a owl:ObjectProperty ;
  rdfs:comment "the bounding box or envelope of the feature" ;
  rdfs:label "has bounding box" ;
  rdfs:range geox:BBox ;
  rdfs:subPropertyOf geo:hasGeometry ;
  skos:example """
auspix:R7430551 a geo:Feature ;
  geox:hasBBox [
      rdf:type geox:BBox ;
      geox:lowerLeft \"<http://www.opengis.net/def/crs/OGC/1.3/CRS84> POINT(131.02880658436214 -25.36980468021464)\"^^geo:wktLiteral ;
      geox:upperRight \"<http://www.opengis.net/def/crs/OGC/1.3/CRS84> POINT(131.06995884773661 -25.331112553792963)\"^^geo:wktLiteral ;
    ] ;
  geox:hasCentroid [
      rdf:type sf:Point ;
      geo:asWKT \"POINT(131.0493827160494, -25.350457086495783)\"^^geo:wktLiteral ;
    ] ;
  geo:hasGeometry [
    rdf:type sf:Polygon ;
    geo:asWKT \"POLYGON((131.02880658436214 -25.331112553792963 , 131.06995884773661 -25.331112553792963  , 131.06995884773661 -25.36980468021464 , 131.02880658436214 -25.36980468021464 , 131.02880658436214 -25.331112553792963))\"^^geo:wktLiteral ;
    ] ;
  rdfs:seeAlso <http://ec2-52-63-73-113.ap-southeast-2.compute.amazonaws.com/AusPIX-DGGS-dataset/ausPIX/R7430551> ;
.""" ;
.
geox:hasCentroid
  a owl:ObjectProperty ;
  rdfs:comment "link to the geometric centroid, which is the arithmetic mean position of all the points in the 2-D figure" ;
  rdfs:label "has centroid" ;
  rdfs:range [
      a owl:Class ;
      owl:unionOf (
          <http://www.opengis.net/ont/sf#Point>
          <http://www.opengis.net/ont/gml#Point>
        ) ;
    ] ;
  rdfs:subPropertyOf geo:hasGeometry ;
  skos:example """
auspix:R7430551 a geo:Feature ;
  geox:hasCentroid [
      rdf:type sf:Point ;
      geo:asWKT \"POINT(131.0493827160494, -25.350457086495783)\"^^geo:wktLiteral ;
    ] ;
  geo:hasGeometry [
    rdf:type sf:Polygon ;
    geo:asWKT \"POLYGON((131.02880658436214 -25.331112553792963 , 131.06995884773661 -25.331112553792963  , 131.06995884773661 -25.36980468021464 , 131.02880658436214 -25.36980468021464 , 131.02880658436214 -25.331112553792963))\"^^geo:wktLiteral ;
    ] ;
  rdfs:seeAlso <http://ec2-52-63-73-113.ap-southeast-2.compute.amazonaws.com/AusPIX-DGGS-dataset/ausPIX/R7430551> ;
.""" ;
.
geox:hasLength
  a owl:ObjectProperty ;
  rdfs:domain geo:SpatialObject ;
  rdfs:label "has length" ;
  rdfs:range geox:SpatialMeasure ;
  skos:definition "The length of a spatial object, expressed as a scaled number" ;
  skos:example """
my:road456
  :hasLength [
    data:uncertainty 5.0 ;
    data:unit <http://qudt.org/vocab/unit/M> ;
    data:value 234.0 ;
  ] ;
.""" ;
.
geox:hasLengthM
  a owl:ObjectProperty ;
  rdfs:label "has length in m" ;
  rdfs:range [
      a owl:Class ;
      rdfs:subClassOf data:QuantitativeMeasure ;
      rdfs:subClassOf [
          a owl:Restriction ;
          owl:hasValue <http://qudt.org/vocab/unit/M> ;
          owl:onProperty data:unit ;
        ] ;
    ] ;
  rdfs:subPropertyOf geox:hasLength ;
  skos:definition "The length of a spatial object in metres" ;
  skos:example """
my:road456
  :hasLengthM [
    data:value 234.0 ;
  ] ;
.""" ;
.
geox:hasResolution
  a owl:ObjectProperty ;
  rdfs:domain geo:Geometry ;
  rdfs:label "has spatial resolution" ;
  rdfs:range data:QuantitativeMeasure ;
  skos:altLabel "spatial resolution" ;
  skos:definition "The spatial resolution of the Geometry object, expressed as a linear measurement." ;
  skos:example """
my:image456
  :hasResolution [
    data:unit <http://qudt.org/vocab/unit/M> ;
    data:value 30.0 ;
  ] ;
.""" ;
  skos:usageNote "This is only to be used for geoGeometry objects. If you want to talk about the precision of things like area, that's regular QUDT business." ;
.
geox:hasResolutionM
  a owl:ObjectProperty ;
  rdfs:domain geo:Geometry ;
  rdfs:label "has spatial resolution in metres" ;
  rdfs:range [
      a owl:Class ;
      rdfs:subClassOf data:QuantitativeMeasure ;
      rdfs:subClassOf [
          a owl:Restriction ;
          owl:hasValue <http://qudt.org/vocab/unit/M> ;
          owl:onProperty data:unit ;
        ] ;
    ] ;
  rdfs:subPropertyOf geox:hasResolution ;
  skos:altLabel "spatial resolution" ;
  skos:definition "The spatial resolution of the Geometry object, expressed as a linear distance in metres" ;
  skos:example """
my:image456
  :hasResolutionM [
    data:value 30.0 ;
  ] ;
.""" ;
  skos:usageNote "This is only to be used for geoGeometry objects. If you want to talk about the precision of things like area, that's regular QUDT or DQV business" ;
.
geox:hasVolume
  a owl:ObjectProperty ;
  rdfs:domain geo:SpatialObject ;
  rdfs:label "has volume" ;
  rdfs:range geox:SpatialMeasure ;
  skos:definition "The volume of a spatial object, expressed as a scaled number" ;
  skos:example """
my:swimmingPool99
  :hasVolume [
    data:unit <http://qudt.org/vocab/unit/M3> ;
    data:value 3050.0 ;
  ] ;
.""" ;
.
geox:hasVolumeM3
  a owl:ObjectProperty ;
  rdfs:label "has volume in m3" ;
  rdfs:range [
      a owl:Class ;
      rdfs:subClassOf data:QuantitativeMeasure ;
      rdfs:subClassOf [
          a owl:Restriction ;
          owl:hasValue <http://qudt.org/vocab/unit/M3> ;
          owl:onProperty data:unit ;
        ] ;
    ] ;
  rdfs:subPropertyOf geox:hasVolume ;
  skos:definition "The volume of a spatial object in cubic-metres" ;
  skos:example """
my:swimmingPool99
  :hasVolumeM3 [
    data:value 3050.0 ;
  ] ;
.""" ;
.
geox:inCRS
  a owl:ObjectProperty ;
  rdfs:label "In Coordinate Reference System" ;
  skos:definition """Geometry, position or measure is defined or computed using this CRS. 
The CRS should be denoted by a URI Reference to a CRS definition, e.g. https://www.opengis.net/def/crs/EPSG/0/4326""" ;
.
geox:isGeometryOf
  a owl:ObjectProperty ;
  rdfs:domain geo:Geometry ;
  rdfs:label "is geometry of" ;
  rdfs:range geo:Feature ;
  owl:inverseOf geo:hasGeometry ;
  skos:definition "link from a geometry object to the feature(s) for which it is a geometry" ;
.
geox:lowerLeft
  a owl:DatatypeProperty ;
  rdfs:comment "position of lower-left corner of box, expressed as a POINT. " ;
  rdfs:domain geox:BBox ;
  rdfs:label "lower-left" ;
  rdfs:range rdfs:Literal ;
  skos:example """
 <>  geox:lowerLeft \"<http://www.opengis.net/def/crs/OGC/1.3/CRS84> POINT(138 -29.5)\"^^geo:wktLiteral .

 <>  geox:lowerLeft \"POINT(138 -29.5)\"^^geo:wktLiteral .""" ;
.
geox:transitiveSfOverlap
  a owl:DeprecatedProperty ;
  a owl:ObjectProperty ;
  rdfs:comment "The domain object overlaps (geo:sfOverlaps) the range object by virtue of both objects containing (geo:sfContains) an intermediary object." ;
  rdfs:domain geo:SpatialObject ;
  rdfs:prefLabel "transitive Simple Features overlaps" ;
  rdfs:range geo:SpatialObject ;
  rdfs:subPropertyOf geo:sfOverlaps ;
  owl:deprecated true ;
  owl:propertyChainAxiom (
      geo:sfContains
      geo:sfWithin
    ) ;
  skos:altLabel "proportional overlap" ;
  skos:editorialNote "This property is not needed - it is not a true sub-property, it is a rule to infer overlap from the existence of a common contained feature ... it is actually more like a record of the _provenance_ of an sfOverlaps property. That information would be better managed as part of a linking statement. " ;
  skos:usageNote "if ex:A geo:sfContains ex:X and ex:B geo:sfContains :ex:X, using the declaration of geo:sfWithin in this ontology with an owl:inverseOf to geo:sfOverlaps, we can interpret the second triple as ex:X geo:sfWithin :B and then ex:A geo:sf:Overlaps ex:B with proportionally, being contained in the relative areas of A, B & X" ;
.
geox:upperRight
  a owl:DatatypeProperty ;
  rdfs:comment "position of upper-right corner of box, expressed as a POINT. " ;
  rdfs:domain geox:BBox ;
  rdfs:label "upper-right" ;
  rdfs:range rdfs:Literal ;
  skos:example """
<>      geox:upperRight \"POINT(155 -9)\"^^geo:wktLiteral .

<>      geox:upperRight \"<http://www.opengis.net/def/crs/OGC/1.3/CRS84> POINT(155 -9)\"^^geo:wktLiteral .
""" ;
.
<https://orcid.org/0000-0002-3884-3420>
  a owl:NamedIndividual ;
  a sdo:Person ;
  sdo:affiliation [
      sdo:identifier "http://catalogue.linked.data.gov.au/org/csiro"^^xsd:anyURI ;
      sdo:name "CSIRO" ;
    ] ;
  sdo:email <mailto:simon.cox@csiro.au> ;
  sdo:identifier "https://orcid.org/0000-0002-3884-3420"^^xsd:anyURI ;
  sdo:name "Simon J D Cox" ;
  sdo:subjectOf <https://people.csiro.au/C/S/simon-cox> ;
.
<https://orcid.org/0000-0002-8742-7730>
  a owl:NamedIndividual ;
  a sdo:Person ;
  sdo:affiliation [
      sdo:identifier "https://surroundaustralia.com/"^^xsd:anyURI ;
      sdo:name "Surround Australia" ;
    ] ;
  sdo:email <mailto:nicholas.car@surroundaustralia.com> ;
  sdo:identifier "https://orcid.org/0000-0002-8742-7730"^^xsd:anyURI ;
  sdo:name "Nicholas J Car" ;
.
<https://ror.org/03qn8fb07>
  a sdo:Organization ;
  sdo:name "CSIRO" ;
  sdo:url <https://www.csiro.au> ;
.
